ironfleet/src/Dafny/Distributed/Protocol/RSL/FailureProof/TopLevel/FailureProof.i.dfy
@@ -93,31 +93,4 @@ lemma RSLTopLevel(tglb:seq<TimestampedRslState>, opn:OperationNumber)
 }
 
 
-/*****************************************************************************************
-*                                  Misc Definitions                                      *
-*****************************************************************************************/
-
-
-
-
-predicate InFailover(ts:TimestampedRslState) 
-    requires |ts.t_replicas| > 2
-{
-    ts.t_replicas[1].v.replica.proposer.election_state.current_view == Ballot(1,0)
-}
-
-predicate InPhase1(ts:TimestampedRslState) 
-    requires |ts.t_replicas| > 2
-{
-    && ts.t_replicas[1].v.replica.proposer.election_state.current_view == Ballot(1,1)
-    && ts.t_replicas[1].v.replica.proposer.current_state != 2
-}
-
-predicate InPhase2(ts:TimestampedRslState) 
-    requires |ts.t_replicas| > 2
-{
-    && ts.t_replicas[1].v.replica.proposer.election_state.current_view == Ballot(1,1)
-    && ts.t_replicas[1].v.replica.proposer.current_state == 2
-}
-
 }
